src/QUIC.Impl.Lemmas.fsti
@@ -1,1 +1,0 @@
-module QUIC.Impl.Lemmas
